MirrorCharge!/src/CancellerTac.v
@@ -1,0 +1,189 @@
+Require Import MirrorCore.SymI.
+Require Import MirrorCore.EnvI.
+Require Import MirrorCore.Ext.Expr.
+Require Import MirrorCore.Ext.ExprUnifySyntactic.
+Require Import MirrorCore.Ext.FMapSubst.
+(* Charge *)
+Require Import ILogic BILogic.
+(* MirrorCharge *)
+Require Import BILNormalize OrderedCanceller SynSepLog.
+Require Import SepLogFold.
+
+Set Implicit Arguments.
+Set Strict Implicit.
+
+Section ordered_cancel_tac.
+  Variable ts : types.
+  Variable func : Type.
+  Variable RSym_func : RSym (typD ts) func.
+  Variable RSymOk_func : RSymOk RSym_func.
+  Variable tySL : typ.
+
+  Let subst := FMapSubst.SUBST.subst func.
+  Local Instance Subst_subst : Subst.Subst subst (expr func) :=
+    @FMapSubst.SUBST.Subst_subst _.
+  Local Instance SubstOk_subst : @Subst.SubstOk subst (expr func) _ (typD ts) _ _ :=
+    @FMapSubst.SUBST.SubstOk_subst _ _ _.
+
+  Definition eprovePure : subst -> expr func -> option subst :=
+    fun _ _ => None.
+
+  Definition doUnifySepLog (fuel : nat) (tus tvs : EnvI.tenv typ)
+  : subst -> expr func -> expr func -> option subst :=
+    fun s e e' =>
+      @exprUnify subst ts func _ _ fuel tus tvs 0 s e e' tySL.
+
+  Definition order : conjunctives func -> Conjuncts func :=
+    @simple_order _.
+
+  Variable ILogicOps_SL : ILogicOps (typD ts nil tySL).
+  Variable ILogic_SL : ILogic (typD ts nil tySL).
+  Variable BILOperators_SL : BILOperators (typD ts nil tySL).
+  Variable BILogic_SL : BILogic (typD ts nil tySL).
+  Variable SSL : SynSepLog func.
+  Variable SSLO : SynSepLogOk _ _ _ _ SSL.
+
+  Lemma WellTyped_env_join_env
+  : forall tus (us : HList.hlist (typD ts nil) tus),
+      WellTyped_env tus (EnvI.join_env us).
+  Proof.
+    induction tus; intros; red.
+    { rewrite (HList.hlist_eta us). simpl. constructor. }
+    { rewrite (HList.hlist_eta us). simpl; constructor; auto. apply IHtus. }
+  Qed.
+
+  Theorem unifySepLogOk tus tvs
+  : unifySepLog_spec SubstOk_subst (doUnifySepLog 100 tus tvs) tySL tus tvs.
+  Proof.
+    specialize exprUnify_sound; intro unifyOk.
+    do 2 red in unifyOk.
+    red. unfold doUnifySepLog.
+    intros.
+    specialize (unifyOk subst ts func _ _ _ _ 100 tus tvs e e' s s' tySL nil H0 H1 H2 H).
+    destruct unifyOk.
+    split; auto.
+    intros.
+    specialize (H4 (EnvI.join_env us) (EnvI.join_env vs)).
+    apply H4 in H5; eauto using WellTyped_env_join_env.
+    destruct H5. specialize (H6 nil).
+    split; auto.
+    apply H6. constructor.
+  Qed.
+
+  Theorem eprovePureOk tus tvs
+  : eprovePure_spec SubstOk_subst eprovePure tySL ILogicOps_SL tus tvs.
+  Proof.
+    red. inversion 1.
+  Qed.
+
+  Definition the_canceller (sls : SepLogSpec func) tus tvs (lhs rhs : expr func) s :=
+    let lhs_norm := normalize sls lhs tus tvs in
+    let rhs_norm := normalize sls rhs tus tvs in
+    let '(lhs',rhs',s') :=
+        ordered_cancel (doUnifySepLog 100 tus tvs) eprovePure
+                       (simple_order (func:=func)) lhs_norm rhs_norm s
+    in (conjunctives_to_expr SSL lhs', conjunctives_to_expr SSL rhs', s').
+
+  Variable sls : SepLogSpec func.
+  Hypothesis slsOk : @SepLogSpecOk ts _ _ tySL sls _ _.
+
+  Require Import ExtLib.Tactics.
+
+  Ltac forward_reason :=
+    repeat match goal with
+             | H : ?X , H' : ?X -> _ |- _ =>
+               match type of X with
+                 | Prop => specialize (H' H)
+               end
+             | H : ?X -> _ |- _ =>
+               match type of X with
+                 | Prop => let Z := fresh in
+                           assert (Z : X) by eauto ;
+                             specialize (H Z) ; clear Z
+               end
+             | H : _ /\ _ |- _ => destruct H
+             | H : exists x, _ |- _ => destruct H
+           end.
+
+  Local Instance PureOp_pure : @Pure.PureOp (typD ts nil tySL) := slsOk.(_PureOp).
+  Local Instance Pure_pure : @Pure.Pure (typD ts nil tySL) _ _ _ := slsOk.(_Pure).
+
+  Theorem the_cancellerOk (Pure_true : Pure.pure ltrue)
+  : forall us vs lhs rhs lhs' rhs' sub,
+      the_canceller sls (typeof_env us) (typeof_env vs) lhs rhs (@FMapSubst.SUBST.subst_empty _) = (lhs', rhs', sub) ->
+      match exprD us vs lhs' tySL
+          , exprD us vs rhs' tySL
+      with
+        | Some lhs , Some rhs =>
+          Subst.substD us vs sub /\
+            lhs |-- rhs
+        | None , None => True
+        | _ , _ => False
+      end ->
+      match exprD us vs lhs tySL
+          , exprD us vs rhs tySL
+      with
+        | Some lhs , Some rhs =>
+          lhs |-- rhs
+        | _ , _ => True
+      end.
+  Proof.
+    unfold the_canceller. intros.
+    consider (split_env us); intros.
+    generalize (@normalizeOk ts func _ _ _ _ _ _ sls slsOk SSL SSLO lhs us (typeof_env vs)).
+    generalize (@normalizeOk ts func _ _ _ _ _ _ sls slsOk SSL SSLO rhs us (typeof_env vs)).
+    consider (split_env vs); intros.
+    consider (ordered_cancel
+              (doUnifySepLog 100 (typeof_env us) (typeof_env vs)) eprovePure
+              (simple_order (func:=func))
+              (normalize sls lhs (typeof_env us) (typeof_env vs))
+              (normalize sls rhs (typeof_env us) (typeof_env vs))
+              (SUBST.subst_empty func)).
+    destruct p; intros.
+    assert (typeof_env us = x).
+    { unfold typeof_env. rewrite <- split_env_projT1.
+      rewrite H1. reflexivity. }
+    assert (typeof_env vs = x0).
+    { unfold typeof_env. rewrite <- split_env_projT1.
+      rewrite H2. reflexivity. }
+    rewrite H6 in *.
+    rewrite H7 in *.
+    generalize (@ordered_cancelOk ts func RSym_func subst Subst_subst _
+                             (doUnifySepLog 100 x x0)
+                             eprovePure tySL ILogicOps_SL BILOperators_SL _ _ x x0
+                             (@unifySepLogOk x x0)
+                             (@eprovePureOk x x0)
+                             SSL SSLO _ _ Pure_true
+                             (@simple_order func)
+                             (@simple_orderOk ts func _ tySL _ _ _ _ SSL SSLO _)
+                             h
+                             (normalize sls lhs x x0)
+                             (normalize sls rhs x x0)
+                             (@FMapSubst.SUBST.subst_empty _)
+                             c c0 s H).
+    repeat match goal with
+             | _ : context [ normalize ?A ?B ?C ?D ] |- _ =>
+               generalize dependent (normalize A B C D); intros
+           end.
+    unfold exprD in *.
+    rewrite H2 in *.
+    inv_all; subst.
+    assert (us = join_env h).
+    { apply split_env_projT2_join_env. auto. }
+    rewrite <- H5 in *.
+    forward.
+    assert (Subst.WellTyped_subst (typeof_env us) (typeof_env vs)
+          (SUBST.subst_empty func)) by eapply Subst.WellTyped_empty.
+    forward_reason.
+    specialize (H14 h0).
+    specialize (H7 h0).
+    specialize (H10 h0).
+    assert (vs = join_env h0).
+    { apply split_env_projT2_join_env. auto. }
+    rewrite <- H16 in *.
+    forward_reason.
+    rewrite H7. rewrite H10. assumption.
+  Qed.
+End ordered_cancel_tac.
+
+(* Check the_cancellerOk. *)
